Finish proof skeleton

linking/safe_clight_rc.v
@@ -15,6 +15,7 @@ Require Import Clight_eff.
 Require Import sepcomp. Import SepComp.
 Require Import arguments.
 
+Require Import pred_lemmas.
 Require Import core_semantics_tcs.
 Require Import rc_semantics.
 Require Import effect_simulations. Import SM_simulation.
@@ -45,11 +46,26 @@ Definition cl_state_inv (c : RC.state CL_core) (m : mem) e te :=
         {subset getBlocks [:: v] <= RC.reach_set ge c m}
   ].
 
+Fixpoint cl_cont_inv (c : RC.state CL_core) (k : cont) (m : mem) := 
+  match k with
+    | Kstop => True
+    | Kseq s k' => cl_cont_inv c k' m
+    | Kloop1 s1 s2 k' => cl_cont_inv c k' m
+    | Kloop2 s1 s2 k' => cl_cont_inv c k' m
+    | Kswitch k' => cl_cont_inv c k' m
+    | Kcall oid f e te k' => [/\ cl_state_inv c m e te & cl_cont_inv c k' m]
+  end.
+
 Definition cl_core_inv (c : RC.state CL_core) (m : mem) := 
   match RC.core c with
-    | CL_State f s k e te => cl_state_inv c m e te
-    | CL_Callstate f args k => {subset getBlocks args <= RC.reach_set ge c m}
-    | CL_Returnstate v k => {subset getBlocks [:: v] <= RC.reach_set ge c m}
+    | CL_State f s k e te => 
+        [/\ cl_state_inv c m e te & cl_cont_inv c k m]
+    | CL_Callstate f args k => 
+        [/\ {subset getBlocks args <= RC.reach_set ge c m} 
+          & cl_cont_inv c k m]
+    | CL_Returnstate v k => 
+        [/\ {subset getBlocks [:: v] <= RC.reach_set ge c m}
+          & cl_cont_inv c k m]
   end.
 
 Lemma getBlocksP l b : reflect (exists ofs, List.In (Vptr b ofs) l) (b \in getBlocks l).
@@ -212,6 +228,39 @@ move=> H H2 b'; case/getBlocksP=> ofs'; case=> //; case=> <- _; case: H2=> //.
   by exists ofs0; constructor. }
 Qed.
 
+Lemma eval_exprlist_reach' c m e te aa tys vv : 
+  cl_state_inv c m e te ->    
+  eval_exprlist ge e te m aa tys vv -> 
+  {subset getBlocks vv <= RC.reach_set ge c m}.
+Proof.
+move=> H; elim=> // a bl ty tyl v1 v2 vl H2 H3 H4 H5.
+move=> b; case/getBlocksP=> ofs; case.
++ move=> Heq; subst v2.
+apply: (eval_expr_reach' H H2).
+apply: (sem_cast_getBlocks H3). 
+by apply/getBlocksP; exists ofs; constructor.
++ move=> H6; apply: H5; clear -H6.
+elim: vl H6=> // a vl' H7; case.
+by move=> Heq; subst a; apply/getBlocksP; exists ofs; constructor.
+by move=> H8; apply/getBlocksP; exists ofs; right.
+Qed.
+
+Lemma freelist_effect_reach b ofs f k e te args rets locs m :
+  let: c := {|
+     RC.core := CL_State f (Sreturn None) k e te;
+     RC.args := args;
+     RC.rets := rets;
+     RC.locs := locs |} in
+   FreelistEffect m (blocks_of_env e) b ofs ->
+   cl_state_inv c m e te -> 
+   RC.reach_set ge c m b.
+Admitted.
+
+Lemma builtin_effects_reach (c : RC.state CL_core) ef vargs m b ofs :
+  BuiltinEffects.BuiltinEffect ge ef vargs m b ofs -> 
+  RC.reach_set ge c m b.
+Admitted.
+
 Lemma eval_expr_reach c m a v : 
   cl_core_inv c m -> 
   match RC.core c with 
@@ -222,9 +271,84 @@ Lemma eval_expr_reach c m a v :
   end.
 Proof.
 rewrite /cl_core_inv; case: (RC.core c)=> //. 
-by move=> f s k e te; apply: eval_expr_reach'.
+by move=> f s k e te []H _; move: H; apply: eval_expr_reach'.
 Qed.
 
+Lemma external_call_reach l (ef : external_function) vargs m t v m' : 
+  ~BuiltinEffects.observableEF hf ef -> 
+  external_call ef ge vargs m t v m' -> 
+  {subset getBlocks vargs <= REACH m l} -> 
+  {subset getBlocks [:: v] <= [predU REACH m l & freshloc m m']}.
+Admitted.
+
+Lemma cont_inv_call_cont c k m : 
+  cl_cont_inv c k m -> 
+  cl_cont_inv c (call_cont k) m.
+Proof. by elim: k. Qed.
+
+Lemma cont_inv_find_label c lbl s k s' k' m :
+  cl_cont_inv c k m -> 
+  find_label lbl s (call_cont k) = Some (s', k') -> 
+  cl_cont_inv c k' m.
+Admitted.
+
+Lemma cont_inv_freshlocs c0 c' k m m' args rets locs :
+   let: c := {|RC.core := c0;
+               RC.args := args;
+               RC.rets := rets;
+               RC.locs := locs |} in
+   cl_cont_inv c k m -> 
+   cl_cont_inv
+        {|RC.core := c';
+          RC.args := args;
+          RC.rets := rets;
+          RC.locs := fun b : block =>
+            locs b || freshloc m m' b || RC.reach_set ge c m b |} k m'.
+Proof.
+elim: k=> //= _ _ e te k' H []H2 H3; split=> //.
++ clear -H2; move: H2; rewrite /cl_state_inv; case=> He Hte; split.
+move=> x b ty H; apply/orP; right; apply/orP; right. 
+by apply: REACH_nil; apply: (He _ _ _ H).
+move=> x v H b H2; apply: REACH_nil; apply/orP; right; apply/orP; right.
+by apply: (Hte _ _ H).
++ by apply: H.
+Qed.
+
+Lemma state_inv_freshlocs c0 c' m m' args rets locs e te :
+  let: c := {|RC.core := c0;
+              RC.args := args;
+              RC.rets := rets;
+              RC.locs := locs |} in
+  cl_state_inv c m e te ->
+  cl_state_inv {|
+     RC.core := c';
+     RC.args := args;
+     RC.rets := rets;
+     RC.locs := fun b : block =>
+       RC.locs c b || freshloc m m' b || RC.reach_set ge c m b |} m' e te.
+Proof.
+case=> He Hte; split.
++ move=> x b ty H; apply/orP; right; apply/orP; right.
+by apply: REACH_nil; apply: (He _ _ _ H).
++ move=> x v H b H2; apply: REACH_nil; apply/orP; right; apply/orP; right.
+by apply: (Hte _ _ H _ H2).
+Qed.
+
+Lemma function_entry1_state_inv (c0 : RC.state CL_core) c1 f vargs m e te m' args locs rets : 
+  let: c := {| RC.core := c0;
+               RC.args := args;
+               RC.rets := rets;
+               RC.locs := locs |} in
+  let: c' := {| RC.core := c1;
+               RC.args := args;
+               RC.rets := rets;
+               RC.locs := fun b0 : block =>
+                RC.locs c b0 || freshloc m m' b0 || RC.reach_set ge c m b0 |} in
+  {subset getBlocks vargs <= RC.reach_set ge c m} -> 
+  function_entry1 f vargs m e te m' -> 
+  cl_state_inv c' m' e te.
+Admitted.
+        
 Lemma rc_safe z c m :
   cl_core_inv c m -> 
   (forall n, safeN clsem espec ge n z (RC.core c) m) -> 
@@ -274,23 +398,26 @@ move: step Inv Hsafe Hatext Hhlt; case: c=> /= core args rets locs; case.
   + case/andP; case/andP=> Heq _ _.
     have Heq': loc = b by rewrite /eq_block in Heq; case: (Coqlib.peq loc b) Heq.
     subst loc; move {Heq}; rewrite /cl_core_inv /= in Inv.
+    case: Inv=> Inv Inv2.
     by apply: (eval_lvalue_reach Inv H); apply/getBlocksP; exists ofs; constructor.
   + case/andP; case/andP=> Heq _ _.
     have Heq': loc = b by rewrite /eq_block in Heq; case: (Coqlib.peq b loc) Heq.
     subst loc; move {Heq}; rewrite /cl_core_inv /= in Inv.
+    case: Inv=> Inv Inv2.
     by apply: (eval_lvalue_reach Inv H); apply/getBlocksP; exists ofs; constructor. }
   
   { apply: IH=> //.
   (*reestablish invariant*)
   move: Inv; rewrite /cl_core_inv /cl_state_inv /RC.roots /=. 
-  case=> H5 H6; split=> //=.
+  case; case=> H5 H6 Hk; split=> //.
+  split.
   { rewrite /locs''=> x b ty H7.
     move: (H5 _ _ _ H7); case/orP; first by move=> ->.
     by rewrite /= => ->; apply/orP; right. }
   { move=> x v0 H7; move: (H6 _ _ H7)=> H8 b H9; move: (H8 b H9).
     rewrite /locs'' /RC.reach_set /RC.roots /= => H10.
-    by apply: REACH_nil; apply/orP; right; apply/orP; right. } }
-}
+    by apply: REACH_nil; apply/orP; right; apply/orP; right. } 
+  by move: Hk; apply: cont_inv_freshlocs. } }
 
 { move=> f id a k e te m0 v H Inv H2 _ _.
   set (c'' := CL_State f Sskip k e (PTree.set id v te)).
@@ -308,7 +435,8 @@ move: step Inv Hsafe Hatext Hhlt; case: c=> /= core args rets locs; case.
   apply: IH=> //.
   (*reestablish invariant*)
   move: (Inv); rewrite /cl_core_inv /cl_state_inv /RC.roots /=. 
-  case=> He Hte; split=> //=.
+  case; case=> He Hte Hk; split=> //=.
+  split.
   { rewrite /locs''=> x b ty H7.
     move: (He _ _ _ H7); case/orP; first by move=> ->.
     by rewrite /= => ->; apply/orP; right. }
@@ -320,7 +448,7 @@ move: step Inv Hsafe Hatext Hhlt; case: c=> /= core args rets locs; case.
     + rewrite PTree.gso in H7=> //; move: (Hte _ _ H7); move/(_ b H8).
       rewrite /locs'' /RC.reach_set /RC.roots /= => H10.
       by apply: REACH_nil; apply/orP; right; apply/orP; right.  }
-}
+  by move: Hk; apply: cont_inv_freshlocs. } 
 
 { move=> f optid a a1 k e te m0 tyargs tyres vf vargs fd H H2 H3 H4 H5 Inv H6 _ _.
   set (c'' := CL_Callstate fd vargs (Kcall optid f e te k)).
@@ -333,8 +461,540 @@ move: step Inv Hsafe Hatext Hhlt; case: c=> /= core args rets locs; case.
          RC.locs c b || freshloc m0 m0 b || RC.reach_set ge c m0 b).
   exists (RC.mk c'' (RC.args c) (RC.rets c) locs''), m0=> /=; split.
   exists EmptyEffect; split; first by econstructor; eauto.
+  split=> //. 
+
+  apply: IH=> //.
+  (*reestablish invariant*)
+  case: Inv=> Inv Hk.
+  move: (Inv); rewrite /cl_core_inv /cl_state_inv /RC.roots /=.                        
+  case=> He Hte //; split. 
+  move=> b H7; move: (eval_exprlist_reach' Inv H3).
+  move/(_ b H7); rewrite /locs'' /RC.reach_set /RC.roots /= => H10.
+  by apply: REACH_nil; apply/orP; right; apply/orP; right. 
+  split; last by move: Hk; apply: cont_inv_freshlocs. 
+  by move: Inv; apply: state_inv_freshlocs. }
+
+{ move=> f optid ef tyargs a1 k e te m0 vargs t vres m0' H2 H3 H4 Inv H6 _ _.
+  set (c'' := CL_State f Sskip k e (set_opttemp optid vres te)).
+  set (c := {|
+          RC.core := CL_State f (Sbuiltin optid ef tyargs a1) k e te;
+          RC.args := args;
+          RC.rets := rets;
+          RC.locs := locs |}).
+  set (locs'' :=  fun b : block =>
+         RC.locs c b || freshloc m0 m0' b || RC.reach_set ge c m0 b).
+  exists (RC.mk c'' (RC.args c) (RC.rets c) locs''), m0'=> /=; split.
+  exists (BuiltinEffects.BuiltinEffect ge ef vargs m0); split; first by econstructor; eauto.
+  split=> //; first by apply: builtin_effects_reach.
+
+  apply: IH=> //.
+  (*reestablish invariant*)
+  case: Inv=> Inv Hk.
+  move: (Inv); rewrite /cl_core_inv /cl_state_inv /RC.roots /=. 
+  case=> He Hte; split=> //=.
+  split.
+  { rewrite /locs''=> x b ty H7.
+    move: (He _ _ _ H7); case/orP; first by move=> ->.
+    by rewrite /= => ->; apply/orP; right. }
+  { rewrite /c'' /locs'' /c /set_opttemp /=; move {locs'' c c''}.
+    move {Hk}; case: optid Inv H6 Hte.
+    { move=> a Inv H6 Hte x v.
+      move: (eval_exprlist_reach' Inv H2)=> H7.
+      move: (external_call_reach H4 H3 H7)=> H8.
+      case: (ident_eq a x)=> Heq H9.
+      + subst x; rewrite PTree.gss in H9; case: H9=> Heq'; subst vres.
+        move=> b H9; move: (H8 _ H9); rewrite in_predU; case/orP=> H10.
+        by apply: REACH_nil; apply/orP; right; apply/orP; right.
+        by apply: REACH_nil; apply/orP; right; apply/orP; left; apply/orP; right.
+      + rewrite PTree.gso in H9.
+        move=> b H10; move: (Hte _ _ H9); move/(_ b H10)=> H11.
+        by apply: REACH_nil; apply/orP; right; apply/orP; right.  
+        by move=> C; apply: Heq; rewrite C. }
+    { move=> Inv H6 Hte x v H7 b H8; move: (Hte _ _ H7); move/(_ b H8)=> H11.
+        by apply: REACH_nil; apply/orP; right; apply/orP; right. } } 
+  by move: Hk; apply: cont_inv_freshlocs. }
+
+{ move=> f s1 s2 k e te m0 Inv Hsafe _ _.
+  set (c'' := CL_State f s1 (Kseq s2 k) e te).
+  set (c := {|
+          RC.core := CL_State f (Ssequence s1 s2) k e te;
+          RC.args := args;
+          RC.rets := rets;
+          RC.locs := locs |}).
+  set (locs'' :=  fun b : block =>
+         RC.locs c b || freshloc m0 m0 b || RC.reach_set ge c m0 b).
+  exists (RC.mk c'' (RC.args c) (RC.rets c) locs''), m0=> /=; split.
+  exists EmptyEffect; split; first by econstructor; eauto.
   split=> //.
-  
-Admitted. (*TODO*)
+
+  apply: IH=> //.
+  case: Inv=> Inv Hk.
+  move: (Inv); rewrite /cl_core_inv /cl_state_inv /RC.roots /=. 
+  case=> He Hte; split=> //=.
+  split.
+  { rewrite /locs''=> x b ty H7.
+    move: (He _ _ _ H7); case/orP; first by move=> ->.
+    by rewrite /= => ->; apply/orP; right. }
+  { rewrite /c'' /locs'' /c /= => x v H7 b' H8; move {locs'' c c''}.
+    apply: REACH_nil; apply/orP; right; apply/orP; right. 
+    by apply: (Hte _ _ H7 _ H8). } 
+  by move: Hk; apply: cont_inv_freshlocs. }
+
+{ move=> f s k e te m0 Inv Hsafe _ _.
+  set (c'' := CL_State f s k e te).
+  set (c := {|
+          RC.core := CL_State f Sskip (Kseq s k) e te;
+          RC.args := args;
+          RC.rets := rets;
+          RC.locs := locs |}).
+  set (locs'' :=  fun b : block =>
+         RC.locs c b || freshloc m0 m0 b || RC.reach_set ge c m0 b).
+  exists (RC.mk c'' (RC.args c) (RC.rets c) locs''), m0=> /=; split.
+  exists EmptyEffect; split; first by econstructor; eauto.
+  split=> //.
+
+  apply: IH=> //.
+  case: Inv=> Inv Hk.
+  move: (Inv); rewrite /cl_core_inv /cl_state_inv /RC.roots /=. 
+  case=> He Hte; split=> //=.
+  split.
+  { rewrite /locs''=> x b ty H7.
+    move: (He _ _ _ H7); case/orP; first by move=> ->.
+    by rewrite /= => ->; apply/orP; right. }
+  { rewrite /c'' /locs'' /c /= => x v H7 b' H8; move {locs'' c c''}.
+    apply: REACH_nil; apply/orP; right; apply/orP; right. 
+    by apply: (Hte _ _ H7 _ H8). } 
+  by move: Hk; apply: cont_inv_freshlocs. }
+
+{ move=> f s k e te m0 Inv Hsafe _ _.
+  set (c'' := CL_State f Scontinue k e te).
+  set (c := {|
+          RC.core := CL_State f Scontinue (Kseq s k) e te;
+          RC.args := args;
+          RC.rets := rets;
+          RC.locs := locs |}).
+  set (locs'' :=  fun b : block =>
+         RC.locs c b || freshloc m0 m0 b || RC.reach_set ge c m0 b).
+  exists (RC.mk c'' (RC.args c) (RC.rets c) locs''), m0=> /=; split.
+  exists EmptyEffect; split; first by econstructor; eauto.
+  split=> //.
+
+  apply: IH=> //.
+  case: Inv=> Inv Hk.
+  move: (Inv); rewrite /cl_core_inv /cl_state_inv /RC.roots /=. 
+  case=> He Hte; split=> //=.
+  split.
+  { rewrite /locs''=> x b ty H7.
+    move: (He _ _ _ H7); case/orP; first by move=> ->.
+    by rewrite /= => ->; apply/orP; right. }
+  { rewrite /c'' /locs'' /c /= => x v H7 b' H8; move {locs'' c c''}.
+    apply: REACH_nil; apply/orP; right; apply/orP; right. 
+    by apply: (Hte _ _ H7 _ H8). } 
+  by move: Hk; apply: cont_inv_freshlocs. }
+
+{ move=> f s k e te m0 Inv Hsafe _ _.
+  set (c'' := CL_State f Sbreak k e te).
+  set (c := {|
+          RC.core := c'';
+          RC.args := args;
+          RC.rets := rets;
+          RC.locs := locs |}).
+  set (locs'' :=  fun b : block =>
+         RC.locs c b || freshloc m0 m0 b || RC.reach_set ge c m0 b).
+  exists (RC.mk c'' (RC.args c) (RC.rets c) locs''), m0=> /=; split.
+  exists EmptyEffect; split; first by econstructor; eauto.
+  split=> //.
+
+  apply: IH=> //.
+  case: Inv=> Inv Hk.
+  move: (Inv); rewrite /cl_core_inv /cl_state_inv /RC.roots /=. 
+  case=> He Hte; split=> //=.
+  split.
+  { rewrite /locs''=> x b ty H7.
+    move: (He _ _ _ H7); case/orP; first by move=> ->.
+    by rewrite /= => ->; apply/orP; right. }
+  { rewrite /c'' /locs'' /c /= => x v H7 b' H8; move {locs'' c}.
+    apply: REACH_nil; apply/orP; right; apply/orP; right. 
+    by apply: (Hte _ _ H7 _ H8). }
+  by move: Hk; apply: cont_inv_freshlocs. }
+
+{ move=> f a s1 s2 k e te m0 v1 b Heval H2 Inv Hsafe _ _.
+  set (c'' := CL_State f (if b then s1 else s2) k e te).
+  set (c := {|
+          RC.core := c'';
+          RC.args := args;
+          RC.rets := rets;
+          RC.locs := locs |}).
+  set (locs'' :=  fun b : block =>
+         RC.locs c b || freshloc m0 m0 b || RC.reach_set ge c m0 b).
+  exists (RC.mk c'' (RC.args c) (RC.rets c) locs''), m0=> /=; split.
+  exists EmptyEffect; split; first by econstructor; eauto.
+  split=> //.
+
+  apply: IH=> //. 
+  case: Inv=> Inv Hk; split.
+  move: (Inv); rewrite /cl_core_inv /cl_state_inv /RC.roots.
+  case=> He Hte; split=> //=.
+  { rewrite /locs''=> x b' ty H7; move: (He _ _ _ H7); case/orP; first by move=> ->.
+    by rewrite /= => ->; apply/orP; right. }
+  { rewrite /c'' /locs'' /c /= => x v H7 b' H8; move {locs'' c}.
+    by apply: REACH_nil; apply/orP; right; apply/orP; right; apply: (Hte _ _ H7 _ H8). } 
+  by move: Hk; apply: cont_inv_freshlocs. }
+
+{ move=> f s1 s2 k e te m0 Inv Hsafe _ _.
+  set (c'' := CL_State f s1 (Kloop1 s1 s2 k) e te).
+  set (c := {|
+          RC.core := c'';
+          RC.args := args;
+          RC.rets := rets;
+          RC.locs := locs |}).
+  set (locs'' :=  fun b : block =>
+         RC.locs c b || freshloc m0 m0 b || RC.reach_set ge c m0 b).
+  exists (RC.mk c'' (RC.args c) (RC.rets c) locs''), m0=> /=; split.
+  exists EmptyEffect; split; first by econstructor; eauto.
+  split=> //.
+
+  apply: IH=> //. 
+  case: Inv=> Inv Hk; split.
+  move: (Inv); rewrite /cl_core_inv /cl_state_inv /RC.roots.
+  case=> He Hte; split=> //=.
+  { rewrite /locs''=> x b' ty H7; move: (He _ _ _ H7); case/orP; first by move=> ->.
+    by rewrite /= => ->; apply/orP; right. }
+  { rewrite /c'' /locs'' /c /= => x v H7 b' H8; move {locs'' c}.
+    by apply: REACH_nil; apply/orP; right; apply/orP; right; apply: (Hte _ _ H7 _ H8). } 
+  by move: Hk; apply: cont_inv_freshlocs. }
+
+{ move=> f s1 s2 k e te m0 x H Inv Hsafe _ _.
+  set (c'' := CL_State f s2 (Kloop2 s1 s2 k) e te).
+  set (c := {|
+          RC.core := c'';
+          RC.args := args;
+          RC.rets := rets;
+          RC.locs := locs |}).
+  set (locs'' :=  fun b : block =>
+         RC.locs c b || freshloc m0 m0 b || RC.reach_set ge c m0 b).
+  exists (RC.mk c'' (RC.args c) (RC.rets c) locs''), m0=> /=; split.
+  exists EmptyEffect; split; first by econstructor; eauto.
+  split=> //.
+
+  apply: IH=> //. 
+  case: Inv=> Inv Hk; split.
+  move: (Inv); rewrite /cl_core_inv /cl_state_inv /RC.roots.
+  case=> He Hte; split=> //=.
+  { rewrite /locs''=> x' b' ty H7; move: (He _ _ _ H7); case/orP; first by move=> ->.
+    by rewrite /= => ->; apply/orP; right. }
+  { rewrite /c'' /locs'' /c /= => x' v H7 b' H8; move {locs'' c}.
+    by apply: REACH_nil; apply/orP; right; apply/orP; right; apply: (Hte _ _ H7 _ H8). } 
+  by move: Hk; apply: cont_inv_freshlocs. }
+
+{ move=> f s1 s2 k e te m0 Inv Hsafe _ _.
+  set (c'' := CL_State f Sskip k e te).
+  set (c := {|
+          RC.core := c'';
+          RC.args := args;
+          RC.rets := rets;
+          RC.locs := locs |}).
+  set (locs'' :=  fun b : block =>
+         RC.locs c b || freshloc m0 m0 b || RC.reach_set ge c m0 b).
+  exists (RC.mk c'' (RC.args c) (RC.rets c) locs''), m0=> /=; split.
+  exists EmptyEffect; split; first by econstructor; eauto.
+  split=> //.
+
+  apply: IH=> //. 
+  case: Inv=> Inv Hk; split.
+  move: (Inv); rewrite /cl_core_inv /cl_state_inv /RC.roots.
+  case=> He Hte; split=> //=.
+  { rewrite /locs''=> x' b' ty H7; move: (He _ _ _ H7); case/orP; first by move=> ->.
+    by rewrite /= => ->; apply/orP; right. }
+  { rewrite /c'' /locs'' /c /= => x' v H7 b' H8; move {locs'' c}.
+    by apply: REACH_nil; apply/orP; right; apply/orP; right; apply: (Hte _ _ H7 _ H8). } 
+  by move: Hk; apply: cont_inv_freshlocs. }
+
+{ move=> f s1 s2 k e te m0 Inv Hsafe _ _.
+  set (c'' := CL_State f (Sloop s1 s2) k e te).
+  set (c := {|
+          RC.core := c'';
+          RC.args := args;
+          RC.rets := rets;
+          RC.locs := locs |}).
+  set (locs'' :=  fun b : block =>
+         RC.locs c b || freshloc m0 m0 b || RC.reach_set ge c m0 b).
+  exists (RC.mk c'' (RC.args c) (RC.rets c) locs''), m0=> /=; split.
+  exists EmptyEffect; split; first by econstructor; eauto.
+  split=> //.
+
+  apply: IH=> //. 
+  case: Inv=> Inv Hk; split.
+  move: (Inv); rewrite /cl_core_inv /cl_state_inv /RC.roots.
+  case=> He Hte; split=> //=.
+  { rewrite /locs''=> x' b' ty H7; move: (He _ _ _ H7); case/orP; first by move=> ->.
+    by rewrite /= => ->; apply/orP; right. }
+  { rewrite /c'' /locs'' /c /= => x' v H7 b' H8; move {locs'' c}.
+    by apply: REACH_nil; apply/orP; right; apply/orP; right; apply: (Hte _ _ H7 _ H8). } 
+  by move: Hk; apply: cont_inv_freshlocs. }
+
+{ move=> f s1 s2 k e te m0 Inv Hsafe _ _.
+  set (c'' := CL_State f Sskip k e te).
+  set (c := {|
+          RC.core := c'';
+          RC.args := args;
+          RC.rets := rets;
+          RC.locs := locs |}).
+  set (locs'' :=  fun b : block =>
+         RC.locs c b || freshloc m0 m0 b || RC.reach_set ge c m0 b).
+  exists (RC.mk c'' (RC.args c) (RC.rets c) locs''), m0=> /=; split.
+  exists EmptyEffect; split; first by econstructor; eauto.
+  split=> //.
+
+  apply: IH=> //. 
+  case: Inv=> Inv Hk; split.
+  move: (Inv); rewrite /cl_core_inv /cl_state_inv /RC.roots.
+  case=> He Hte; split=> //=.
+  { rewrite /locs''=> x' b' ty H7; move: (He _ _ _ H7); case/orP; first by move=> ->.
+    by rewrite /= => ->; apply/orP; right. }
+  { rewrite /c'' /locs'' /c /= => x' v H7 b' H8; move {locs'' c}.
+    by apply: REACH_nil; apply/orP; right; apply/orP; right; apply: (Hte _ _ H7 _ H8). } 
+  by move: Hk; apply: cont_inv_freshlocs. }
+
+{ move=> f k e te m0 m0' Hfree Inv Hsafe _ _.
+  set (c'' := CL_Returnstate Vundef (call_cont k)).
+  set (c := {|
+          RC.core := c'';
+          RC.args := args;
+          RC.rets := rets;
+          RC.locs := locs |}).
+  set (locs'' :=  fun b : block =>
+         RC.locs c b || freshloc m0 m0' b || RC.reach_set ge c m0 b).
+  exists (RC.mk c'' (RC.args c) (RC.rets c) locs''), m0'=> /=; split.
+  exists (FreelistEffect m0 (blocks_of_env e)); split; first by econstructor; eauto.
+  split=> //.
+
+  case: Inv=> Inv Hk.
+  by move=> b ofs Hfree'; apply: (freelist_effect_reach Hfree' Inv).
+  apply: IH=> //.
+  move: Inv; case=> Hs Hk; split=> //. 
+  apply: cont_inv_call_cont.
+  by move: Hk; apply: cont_inv_freshlocs. }
+
+{ move=> f a k e te m0 v v' m0' Heval Hcast Hfree Inv Hsafe _ _.
+  set (c'' := CL_Returnstate v' (call_cont k)).
+  set (c := {|
+          RC.core := c'';
+          RC.args := args;
+          RC.rets := rets;
+          RC.locs := locs |}).
+  set (locs'' :=  fun b : block =>
+         RC.locs c b || freshloc m0 m0' b || RC.reach_set ge c m0 b).
+  exists (RC.mk c'' (RC.args c) (RC.rets c) locs''), m0'=> /=; split.
+  exists (FreelistEffect m0 (blocks_of_env e)); split; first by econstructor; eauto.
+  split=> //.
+
+  case: Inv=> Inv Hk.
+  by move=> b ofs Hfree'; apply: (freelist_effect_reach Hfree' Inv).
+  apply: IH=> //.
+  move: Inv; case=> Hs Hk; split=> //. 
+  move=> b; move/sem_cast_getBlocks; move/(_ _ _ _ Hcast)=> Hget.
+  move: (eval_expr_reach' Hs Heval Hget)=> H.
+  by apply: REACH_nil; apply/orP; right; apply/orP; right.
+  apply: cont_inv_call_cont.
+  by move: Hk; apply: cont_inv_freshlocs. }
+
+{ move=> f k e te m0 m0' Hcall Hfree Inv Hsafe _ _.
+  set (c'' := CL_Returnstate Vundef k).
+  set (c := {|
+          RC.core := c'';
+          RC.args := args;
+          RC.rets := rets;
+          RC.locs := locs |}).
+  set (locs'' :=  fun b : block =>
+         RC.locs c b || freshloc m0 m0' b || RC.reach_set ge c m0 b).
+  exists (RC.mk c'' (RC.args c) (RC.rets c) locs''), m0'=> /=; split.
+  exists (FreelistEffect m0 (blocks_of_env e)); split; first by econstructor; eauto.
+  split=> //.
+
+  case: Inv=> Inv Hk.
+  by move=> b ofs Hfree'; apply: (freelist_effect_reach Hfree' Inv).
+  apply: IH=> //.
+  move: Inv; case=> Hs Hk; split=> //. 
+  by move: Hk; apply: cont_inv_freshlocs. }
+
+{ move=> f s1 s2 k e te m0 n0 Heval Inv Hsafe _ _.
+  set (c'' := CL_State f (seq_of_labeled_statement (select_switch n0 s2))
+               (Kswitch k) e te).
+  set (c := {|
+          RC.core := c'';
+          RC.args := args;
+          RC.rets := rets;
+          RC.locs := locs |}).
+  set (locs'' :=  fun b : block =>
+         RC.locs c b || freshloc m0 m0 b || RC.reach_set ge c m0 b).
+  exists (RC.mk c'' (RC.args c) (RC.rets c) locs''), m0=> /=; split.
+  exists EmptyEffect; split; first by econstructor; eauto.
+  split=> //.
+
+  apply: IH=> //. 
+  case: Inv=> Inv Hk; split.
+  move: (Inv); rewrite /cl_core_inv /cl_state_inv /RC.roots.
+  case=> He Hte; split=> //=.
+  { rewrite /locs''=> x' b' ty H7; move: (He _ _ _ H7); case/orP; first by move=> ->.
+    by rewrite /= => ->; apply/orP; right. }
+  { rewrite /c'' /locs'' /c /= => x' v H7 b' H8; move {locs'' c}.
+    by apply: REACH_nil; apply/orP; right; apply/orP; right; apply: (Hte _ _ H7 _ H8). } 
+  by move: Hk; apply: cont_inv_freshlocs. }
+
+{ move=> f x k e te m0 Hx Inv Hsafe _ _.
+  set (c'' := CL_State f Sskip k e te).
+  set (c := {|
+          RC.core := c'';
+          RC.args := args;
+          RC.rets := rets;
+          RC.locs := locs |}).
+  set (locs'' :=  fun b : block =>
+         RC.locs c b || freshloc m0 m0 b || RC.reach_set ge c m0 b).
+  exists (RC.mk c'' (RC.args c) (RC.rets c) locs''), m0=> /=; split.
+  exists EmptyEffect; split; first by econstructor; eauto.
+  split=> //.
+
+  apply: IH=> //. 
+  case: Inv=> Inv Hk; split.
+  move: (Inv); rewrite /cl_core_inv /cl_state_inv /RC.roots.
+  case=> He Hte; split=> //=.
+  { rewrite /locs''=> x' b' ty H7; move: (He _ _ _ H7); case/orP; first by move=> ->.
+    by rewrite /= => ->; apply/orP; right. }
+  { rewrite /c'' /locs'' /c /= => x' v H7 b' H8; move {locs'' c}.
+    by apply: REACH_nil; apply/orP; right; apply/orP; right; apply: (Hte _ _ H7 _ H8). } 
+  by move: Hk; apply: cont_inv_freshlocs. }
+
+{ move=> f k e te m0 Inv Hsafe _ _.
+  set (c'' := CL_State f Scontinue k e te).
+  set (c := {|
+          RC.core := c'';
+          RC.args := args;
+          RC.rets := rets;
+          RC.locs := locs |}).
+  set (locs'' :=  fun b : block =>
+         RC.locs c b || freshloc m0 m0 b || RC.reach_set ge c m0 b).
+  exists (RC.mk c'' (RC.args c) (RC.rets c) locs''), m0=> /=; split.
+  exists EmptyEffect; split; first by econstructor; eauto.
+  split=> //.
+
+  apply: IH=> //. 
+  case: Inv=> Inv Hk; split.
+  move: (Inv); rewrite /cl_core_inv /cl_state_inv /RC.roots.
+  case=> He Hte; split=> //=.
+  { rewrite /locs''=> x' b' ty H7; move: (He _ _ _ H7); case/orP; first by move=> ->.
+    by rewrite /= => ->; apply/orP; right. }
+  { rewrite /c'' /locs'' /c /= => x' v H7 b' H8; move {locs'' c}.
+    by apply: REACH_nil; apply/orP; right; apply/orP; right; apply: (Hte _ _ H7 _ H8). } 
+  by move: Hk; apply: cont_inv_freshlocs. }
+
+{ move=> f lbl s k e te m0 Inv Hsafe _ _.
+  set (c'' := CL_State f s k e te).
+  set (c := {|
+          RC.core := c'';
+          RC.args := args;
+          RC.rets := rets;
+          RC.locs := locs |}).
+  set (locs'' :=  fun b : block =>
+         RC.locs c b || freshloc m0 m0 b || RC.reach_set ge c m0 b).
+  exists (RC.mk c'' (RC.args c) (RC.rets c) locs''), m0=> /=; split.
+  exists EmptyEffect; split; first by econstructor; eauto.
+  split=> //.
+
+  apply: IH=> //. 
+  case: Inv=> Inv Hk; split.
+  move: (Inv); rewrite /cl_core_inv /cl_state_inv /RC.roots.
+  case=> He Hte; split=> //=.
+  { rewrite /locs''=> x' b' ty H7; move: (He _ _ _ H7); case/orP; first by move=> ->.
+    by rewrite /= => ->; apply/orP; right. }
+  { rewrite /c'' /locs'' /c /= => x' v H7 b' H8; move {locs'' c}.
+    by apply: REACH_nil; apply/orP; right; apply/orP; right; apply: (Hte _ _ H7 _ H8). } 
+  by move: Hk; apply: cont_inv_freshlocs. }
+
+{ move=> f lbl k e te m0 s' k' Hfnd Inv Hsafe _ _.
+  set (c'' := CL_State f s' k' e te).
+  set (c := {|
+          RC.core := c'';
+          RC.args := args;
+          RC.rets := rets;
+          RC.locs := locs |}).
+  set (locs'' :=  fun b : block =>
+         RC.locs c b || freshloc m0 m0 b || RC.reach_set ge c m0 b).
+  exists (RC.mk c'' (RC.args c) (RC.rets c) locs''), m0=> /=; split.
+  exists EmptyEffect; split; first by econstructor; eauto.
+  split=> //.
+
+  apply: IH=> //. 
+  case: Inv=> Inv Hk; split.
+  move: (Inv); rewrite /cl_core_inv /cl_state_inv /RC.roots.
+  case=> He Hte; split=> //=.
+  { rewrite /locs''=> x' b' ty H7; move: (He _ _ _ H7); case/orP; first by move=> ->.
+    by rewrite /= => ->; apply/orP; right. }
+  { rewrite /c'' /locs'' /c /= => x' v H7 b' H8; move {locs'' c}.
+    by apply: REACH_nil; apply/orP; right; apply/orP; right; apply: (Hte _ _ H7 _ H8). } 
+  move: Hfnd; apply: cont_inv_find_label.
+  by move: Hk; apply: cont_inv_freshlocs. }
+
+{ move=> f vargs k m0 e te m0' Hentry Inv Hsafe _ _.
+  set (c'' := CL_State f (fn_body f) k e te).
+  set (c := {|
+          RC.core := c'';
+          RC.args := args;
+          RC.rets := rets;
+          RC.locs := locs |}).
+  set (locs'' :=  fun b : block =>
+         RC.locs c b || freshloc m0 m0' b || RC.reach_set ge c m0 b).
+  exists (RC.mk c'' (RC.args c) (RC.rets c) locs''), m0'=> /=; split.
+  exists EmptyEffect; split; first by econstructor; eauto.
+  split=> //.
+
+  apply: IH=> //. 
+  case: Inv=> Inv Hk; split.
+  split.
+  { move=> x b ty H.
+    set (c''' := {| RC.core := c''; RC.args := args; RC.rets := rets; RC.locs := locs'' |}).
+    case: (@function_entry1_state_inv c''' (CL_Callstate (Internal f) vargs k) 
+                                  _ _ _ _ _ _ _ _ _ Inv Hentry)=> /=.
+    by move=> He Hte; apply: (He _ _ _ H). }
+  { move=> x v H. 
+    set (c''' := {| RC.core := c''; RC.args := args; RC.rets := rets; RC.locs := locs'' |}).
+    case: (@function_entry1_state_inv c''' (CL_Callstate (Internal f) vargs k) 
+                                  _ _ _ _ _ _ _ _ _ Inv Hentry)=> /=.
+    by move=> He Hte; apply: (Hte _ _ H). }
+  by move: Hk; apply: cont_inv_freshlocs. }
+
+{ move=> v optid f e te k m0 Inv Hsafe _ _.
+  set (c'' := CL_State f Sskip k e (set_opttemp optid v te)).
+  set (c := {|
+          RC.core := c'';
+          RC.args := args;
+          RC.rets := rets;
+          RC.locs := locs |}).
+  set (locs'' :=  fun b : block =>
+         RC.locs c b || freshloc m0 m0 b || RC.reach_set ge c m0 b).
+  exists (RC.mk c'' (RC.args c) (RC.rets c) locs''), m0=> /=; split.
+  exists EmptyEffect; split; first by econstructor; eauto.
+  split=> //.
+
+  apply: IH=> //. 
+  case: Inv=> Inv /= [][]He Hte Hk; split.
+  split.
+  { move=> x b ty H; apply/orP; right; apply/orP; right.
+    by apply: REACH_nil; move: H; apply: He. }
+  { move=> x v0; rewrite /set_opttemp /locs'' /c /c''; move {locs'' c'' c}.
+    case: optid Hsafe Inv Hk He Hte=> a. 
+    case: (ident_eq a x).
+    + move=> Heq Hsafe Inv Hk He Hte; subst x; rewrite PTree.gss.
+      case=> ?; subst v0=> b Hget; apply: REACH_nil; apply/orP; right; apply/orP; right.
+      by apply: (Inv _ Hget).
+    + move=> Hneq Hsafe Inv Hk He Hte; rewrite PTree.gso=> H.
+      move=> b Hget; apply: REACH_nil; apply/orP; right; apply/orP; right.
+      by apply: (Hte _ _ H _ Hget).
+      by subst x. 
+    move=> Inv Hk He Hte H b Hget; apply: REACH_nil; apply/orP; right; apply/orP; right.
+    by apply: (Hte _ _ H _ Hget). } 
+  by move: Hk; apply: cont_inv_freshlocs. }
+
+Qed.
 
 End SafeClightRC. End SAFE_CLIGHT_RC.
